Makefile
@@ -97,10 +97,11 @@ BACKEND=\
   EraseArgs.v \
   Bounds.v Stacklayout.v Stacking.v Stackingproof.v \
   Asm.v Asmgen.v Asmgenproof0.v Asmgenproof1.v Asmgenproof.v \
+	Inlining.v Inliningspec.v Inliningproof.v \
 	AsmFacts.v RawAsmgen.v
 
 #  Tailcall.v Tailcallproof.v \
-#  Inlining.v Inliningspec.v Inliningproof.v \
+
  
 # C front-end modules (in cfrontend/)
 
